src/mitchell/group_theory/quot_group.lean
@@ -1,0 +1,89 @@
+
+import data.set.basic init.function data.equiv init.logic 
+import mitchell.group_theory.coset mitchell.group_theory.subgroup
+
+universes u v w
+variables {α : Type u} {β : Type v} {γ : Type w}
+
+namespace quotient_group
+open is_subgroup coset_notation
+variable [group α]
+
+def norm_equiv (N : set α) (a b : α) := a * b⁻¹ ∈ N
+
+section norm_equiv
+open is_subgroup coset_notation
+variables [group α] (N : set α) [hn : is_normal_subgroup N] (a : α)
+include hn
+
+lemma norm_equiv_mul {a₁ a₂ b₁ b₂ : α} (ha : norm_equiv N a₁ a₂) (hb : norm_equiv N b₁ b₂)
+    : norm_equiv N (a₁ * b₁) (a₂ * b₂) :=
+    begin
+    simp [norm_equiv] at *,
+    have h : (a₁ * N) * a₂⁻¹ = N, {
+        calc
+            (a₁ * N) * a₂⁻¹ = (N * a₁) * a₂⁻¹   : by rw iff.elim_left (normal_iff_eq_cosets N) hn
+            ...             = N * (a₁ * a₂⁻¹)   : by rw rcoset_assoc
+            ...             = N                 : by rw rcoset_mem_rcoset N (a₁ * a₂⁻¹) (ha)
+    },
+    rw ←h,
+    calc
+        a₁ * b₁ * (b₂⁻¹ * a₂⁻¹) = a₁ * (b₁ * b₂⁻¹) * a₂⁻¹   : by simp
+        ...                     ∈ (a₁ * N) * a₂⁻¹           : mem_rcoset a₂⁻¹ (mem_lcoset a₁ hb)
+    end
+
+end norm_equiv
+
+lemma norm_equiv_rel (N : set α) [is_normal_subgroup N] : equivalence (norm_equiv N) :=
+⟨ λ x, calc
+        x * x⁻¹ = (1 : α) : mul_right_inv x
+        ... ∈ N           : one_mem N,
+    λ x y hxy, calc
+      y * x⁻¹ = (x * y⁻¹)⁻¹         : by simp
+      ...     ∈ N                   : inv_mem hxy,
+    λ x y z hxy hyz, calc
+      x * z⁻¹ = (x * y⁻¹) * (y * z⁻¹) : by rw [mul_assoc, inv_mul_cancel_left y z⁻¹]
+      ...   ∈ N                       : mul_mem hxy hyz ⟩
+
+definition quotient_group_setoid {α} [group α] (N : set α) [is_normal_subgroup N] : setoid α := {
+    r := norm_equiv N,
+    iseqv := norm_equiv_rel N
+}
+
+attribute [instance] quotient_group_setoid
+
+def quotient_group {α} [group α] (N : set α) [h : is_normal_subgroup N] := quotient (quotient_group_setoid N)
+
+notation G `/` N := quotient_group N
+
+
+
+-- instance quotient_group_is_group {α} [G : group α] (N : set α) [hs : is_normal_subgroup N] : group (G / N) := {
+--     mul := quotient.lift₂ (λ x y : α, ⟦x*y⟧) (λ x₁ x₂ y₁ y₂ h₁ h₂, quot.sound $
+--     calc
+--         (x₁ * x₂) * (y₁ * y₂)⁻¹ = x₁ * x₂ * (y₂⁻¹ * y₁⁻¹)   : by rw [mul_inv_rev y₁ y₂]
+--         ...                     = x₁ * (x₂ * y₂⁻¹) * y₁⁻¹   : by rw [←mul_assoc, mul_assoc x₁]
+--         ...                     = x₁ * y₁⁻¹ * (x₂ * y₂⁻¹)   : 
+--         ...                     ∈ N                         : sorry
+    
+-- }
+
+
+end quotient_group
+
+open is_subgroup
+open quotient_group
+open function
+
+structure group_isomorphism (β : Type v) (γ : Type w) [group β] [group γ]
+  extends equiv β γ :=
+(hom_fun : is_hom to_fun)
+
+infix ` ≃ₕ `:50 := group_isomorphism
+
+def image' { α β } ( φ : α → β ) := φ '' univ
+
+
+theorem fake_isomorphism_theorem {α} ( G : group α ) ( H : group α ) { φ : α → α } ( h : is_hom φ ) : (image' φ) ≃ₕ (kernel h) := sorry
+
+theorem first_isomorphism_theorem {α β} ( G : group α ) ( H : group β ) { φ : α → β } ( h : is_hom φ ) : (image' φ) ≃ₕ quotient_group (set.univ) (kernel h) := sorry
